

# Solution: CID for H<sub>2</sub>

- 1 “Calculate the HF energy”

$$E_{\text{HF}} = 2h_1 + (11|11) = -1.8310$$

- 2 “Calculate the ground state CID energy”

$$\mathbf{H}_{\text{CID}} = \begin{pmatrix} H_{11} & H_{12} \\ H_{12} & H_{22} \end{pmatrix} = \begin{pmatrix} 2h_1 + (11|11) & (12|12) \\ (12|12) & 2h_2 + (22|22) \end{pmatrix}$$

$$E_{\text{CID}} = \frac{H_{11} + H_{22} \pm \sqrt{(H_{11} - H_{22})^2 + 4H_{12}^2}}{2} = -1.8516 \text{ or } -0.2331$$

- 3 “Calculate the correlation energy”

$$E_c = E_{\text{CID}} - E_{\text{HF}} = -1.8516 - (-1.8310) = -0.0206$$

- 1 Introduction
- 2 Configuration Interaction Methods
- 3 Møller-Plesset Perturbation Theory**
- 4 Configuration Cluster Methods
- 5 Quantum Monte Carlo Methods

# Rayleigh-Schrödinger perturbation theory

Let's assume we want to find  $\Psi_0$  and  $E_0$ , such as

$$(\mathbf{H}^{(0)} + \lambda \mathbf{H}^{(1)})\Psi_0 = E_0 \Psi_0$$

and that we know

$$\mathbf{H}^{(0)}\Psi_n^{(0)} = E_n^{(0)}\Psi_n^{(0)}, \quad n = 0, 1, 2, \dots, \infty$$

Let's expand  $\Psi_0$  and  $E_0$  in term of  $\lambda$ :

$$E_0 = \lambda^0 E_0^{(0)} + \lambda^1 E_0^{(1)} + \lambda^2 E_0^{(2)} + \lambda^3 E_0^{(3)} + \dots$$

$$\Psi_0 = \lambda^0 \Psi_0^{(0)} + \lambda^1 \Psi_0^{(1)} + \lambda^2 \Psi_0^{(2)} + \lambda^3 \Psi_0^{(3)} + \dots$$

such as (intermediate normalization)

$$\langle \Psi_0^{(0)} | \Psi_0^{(0)} \rangle = 1 \quad \langle \Psi_0^{(0)} | \Psi_0^{(k)} \rangle = 0, \quad k = 1, 2, \dots, \infty$$

# Rayleigh-Schrödinger perturbation theory (Part 1)

*“Can you find the equations giving  $E_0^{(0)}$ ,  $E_0^{(1)}$  and  $E_0^{(2)}$ ?”*

# Rayleigh-Schrödinger perturbation theory (Part 1)

*“Can you find the equations giving  $E_0^{(0)}$ ,  $E_0^{(1)}$  and  $E_0^{(2)}$ ?”*

Gathering terms with respect to the power of  $\lambda$ :

$$\lambda^0 : \quad \mathbf{H}^{(0)}\psi_0^{(0)} = E_0^{(0)}\psi_0^{(0)}$$

$$\lambda^1 : \quad \mathbf{H}^{(0)}\psi_0^{(1)} + \mathbf{H}^{(1)}\psi_0^{(0)} = E_0^{(0)}\psi_0^{(1)} + E_0^{(1)}\psi_0^{(0)}$$

$$\lambda^2 : \quad \mathbf{H}^{(0)}\psi_0^{(2)} + \mathbf{H}^{(1)}\psi_0^{(1)} = E_0^{(0)}\psi_0^{(2)} + E_0^{(1)}\psi_0^{(1)} + E_0^{(2)}\psi_0^{(0)}$$

$$\lambda^3 : \quad \mathbf{H}^{(0)}\psi_0^{(3)} + \mathbf{H}^{(1)}\psi_0^{(2)} = E_0^{(0)}\psi_0^{(3)} + E_0^{(1)}\psi_0^{(2)} + E_0^{(2)}\psi_0^{(1)} + E_0^{(3)}\psi_0^{(0)}$$

Using the intermediate normalization, we have

$$\lambda^0 : \quad E_0^{(0)} = \langle \psi_0^{(0)} | \mathbf{H}^{(0)} | \psi_0^{(0)} \rangle$$

$$\lambda^1 : \quad E_0^{(1)} = \langle \psi_0^{(0)} | \mathbf{H}^{(1)} | \psi_0^{(0)} \rangle$$

$$\lambda^2 : \quad E_0^{(2)} = \langle \psi_0^{(0)} | \mathbf{H}^{(1)} | \psi_0^{(1)} \rangle \quad \text{Wigner's (2n+1) rule!}$$

$$\lambda^3 : \quad E_0^{(3)} = \langle \psi_0^{(0)} | \mathbf{H}^{(1)} | \psi_0^{(2)} \rangle = \langle \psi_0^{(1)} | \mathbf{H}^{(1)} - E_0^{(1)} | \psi_0^{(1)} \rangle$$